Change LlvmExecutor module to the Executor class
The program to execute is given to the constructor for the Executor class, and the
executor is passed to SymbolicExecute(). It makes much more sense this way,
with SymbolicExecute() able to execute different programs or even different
instruction sets, based on the argument.

executor.dfy
@@ -7,33 +7,48 @@
 // null), and for "BranchCondition(s)" to return true.
 
 
+type Reg = int  // Index into map of registers, State.regs
+
+// Fields cannot be duplicated, so fields are appended with the instruction.
+datatype Instr =
+  Add(add_dest: Reg, add_op1: Reg, add_op2: Reg)
+| Icmp(icmp_dest: Reg, icmp_op1: Reg, icmp_op2: Reg)
+| Br(br_cond: Reg, br_label1: int, br_label2: int)
+
+datatype State = State(ip: int, regs: map<Reg, IntExpr>) | HaltedState
+
+
 // Implements a basic subset of the LLVM intermediate representation.
 //   http://llvm.org/docs/LangRef.html
-module LlvmExecutor {
-  import opened SatLib : Z3SatLib
+class Executor {
 
-  type Reg = int  // Index into map of registers, State.regs
+  var program: array<Instr>;
 
-  // Fields cannot be duplicated, so fields are appended with the instruction.
-  datatype Instr =
-    Add(add_dest: Reg, add_op1: Reg, add_op2: Reg)
-  | Icmp(icmp_dest: Reg, icmp_op1: Reg, icmp_op2: Reg)
-  | Br(br_cond: Reg, br_label1: int, br_label2: int)
-
-  datatype State = State(ip: int, regs: map<Reg, IntExpr>) | HaltedState
-
-  method program() returns (instrs: array<Instr>)
-    ensures fresh(instrs)
+  constructor (prog: array<Instr>)
+    requires prog != null
+    ensures fresh(this.program)
+    ensures Valid()
+    modifies this
   {
-    instrs := new Instr[4];
-    instrs[0] := Add(0, 1, 2);
-    instrs[1] := Icmp(0, 0, 1);
-    instrs[2] := Br(0, 3, 4);
-    instrs[3] := Add(0, 1, 2);
-    return instrs;
+    this.program := new Instr[prog.Length];
+
+    // Copy prog to program
+    forall i | 0 <= i < prog.Length
+    {
+      program[i] := prog[i];
+    }
   }
 
-  method GetReg(s: State, r: Reg) returns (regExpr: IntExpr)
+  predicate Valid()
+    reads this
+  {
+    program != null
+  }
+
+  method {:opaque} GetReg(s: State, r: Reg) returns (regExpr: IntExpr)
+    requires Valid()
+    ensures Valid()
+
     requires s.State?
   {
     if r in s.regs {
@@ -43,21 +58,24 @@ module LlvmExecutor {
     }
   }
 
-  method GetInitialState() returns (s: State) {
+  method {:opaque} GetInitialState() returns (s: State)
+    requires Valid()
+    ensures Valid()
+  {
     return State(0, map[]);
   }
 
-  method BranchCondition(s: State) returns (cond: SatLib.BoolExpr)
+  method {:opaque} BranchCondition(s: State) returns (cond: SatLib.BoolExpr)
+    requires Valid()
+    ensures Valid()
   {
-    var prog := program();
-
     // If we're halted, or we run out of instructions, it
     // doesn't matter, the children will be halted.
-    if !(s.State? && 0 <= s.ip < prog.Length) {
+    if !(s.State? && 0 <= s.ip < program.Length) {
       return not(getTrueBool());
     }
 
-    match prog[s.ip] {
+    match program[s.ip] {
       case Add(_, _, _) =>
         return getTrueBool();
       case Icmp(_, _, _) =>
@@ -68,17 +86,18 @@ module LlvmExecutor {
     }
   }
 
-  method Execute(s: State) returns (s1: State, s2: State) {
-    var prog := program();
-
+  method {:opaque} Execute(s: State) returns (s1: State, s2: State)
+    requires Valid()
+    ensures Valid()
+  {
     // If we're halted, both children are also halted
-    if !(s.State? && 0 <= s.ip < prog.Length) {
+    if !(s.State? && 0 <= s.ip < program.Length) {
       return HaltedState, HaltedState;
     }
 
     // Return two children states.
     // If not branching, return (state, HaltedState).
-    match prog[s.ip] {
+    match program[s.ip] {
 
       case Add(dest, op1, op2) =>
         var x1 := GetReg(s, op1);
@@ -108,9 +127,11 @@ module LlvmExecutor {
     }
   }
 
-  method IsHalted(s: State) returns (b: bool) {
-    var prog := program();
-    return !(s.State? && 0 <= s.ip < prog.Length);
+  predicate method {:opaque} IsHalted(s: State)
+    requires Valid()
+    reads this
+  {
+    !(s.State? && 0 <= s.ip < program.Length)
   }
 
 }
